src/DICE.Stubs.fst
@@ -3,7 +3,7 @@ module DICE.Stubs
 open Common
 
 open LowStar.BufferOps
-open Lib.IntTypes
+open FStar.Integers
 
 open Spec.Hash.Definitions
 open Hacl.Hash.Definitions
@@ -28,47 +28,63 @@ module HS  = FStar.HyperStack
 module HST = FStar.HyperStack.ST
 
 
+/// An API to get UDS.
+/// REF: None
+assume val get_UDS
+  (size: nat)
+: HST.Stack (uds_t size)
+  (requires fun _ -> True)
+  (ensures  fun h0 uds h1 ->
+      B.live h1 uds)
+
+
+/// Function to load a library from an image path.
+/// REF: None
 assume val loadLibrary
-  (path: B.buffer imagePath)
+  (path: string)
   (hDLL: hinstance)
 : HST.Stack unit
   (requires fun h ->
-      B.live h path
-    /\ B.live h hDLL.addr
-    /\ B.disjoint path hDLL.addr)
+      B.live h hDLL)
   (ensures fun h0 r h1 ->
-      B.modifies (B.loc_buffer hDLL.addr) h0 h1)
+      B.modifies (B.loc_buffer hDLL) h0 h1)
 
-let fpRiotStart =
-  (cdi: cdi_t)
--> HST.Stack unit
-  (requires fun _ -> True)
-  (ensures  fun _ _ _ -> True)
 
+/// Get function pointer from a loaded library by an entry point.
+/// REF: None
 assume val getProcAddress
   (hDLL: hinstance)
-  (entry: entryPoint)
+  (entry: string)
 : fpRiotStart
 
+
+/// Get offset and size of RIoT Invariant Code.
+/// REF: None
 assume val diceGetRiotInfo
   (hDLL: hinstance)
   (offset: B.pointer I.uint_32)
   (riotSize: B.pointer nat)
 : HST.Stack unit
   (requires fun h ->
-      B.live h hDLL.addr
+      B.live h hDLL
     /\ B.live h offset
     /\ B.live h riotSize
-    /\ B.disjoint hDLL.addr offset
-    /\ B.disjoint hDLL.addr riotSize
+    /\ B.disjoint hDLL offset
+    /\ B.disjoint hDLL riotSize
     /\ B.disjoint riotSize offset)
   (ensures  fun h0 _ h1 ->
       B.modifies (B.loc_buffer offset) h0 h1
     /\ B.modifies (B.loc_buffer riotSize) h0 h1)
 
+
+/// REF: void DiceSHA256 (
+///        const uint8_t *buf,
+///        size_t bufSize,
+///        uint8_t *digest
+///      )
 assume val diceSHA256
-  (size : nat)
-  (data: B.lbuffer uint8 size)
+  (#size : nat)
+  (data: B.lbuffer HI.uint8 size)
   (digest: hash_t SHA2_256)
 : HST.Stack unit
   (requires fun h ->
@@ -77,12 +93,26 @@ assume val diceSHA256
     /\ B.disjoint data digest)
   (ensures  fun h0 _ h1 ->
       B.modifies (B.loc_buffer digest) h0 h1)
+///      {
+///          DICE_SHA256_CONTEXT context;
+///          DICE_SHA256_Init(&context);
+///          DICE_SHA256_Update(&context, buf, bufSize);
+///          DICE_SHA256_Final(&context, digest);
+///      }
 
+
+/// REF: void DiceSHA256_2 (
+///        const uint8_t *buf1,
+///        size_t bufSize1,
+///        const uint8_t *buf2,
+///        size_t bufSize2,
+///        uint8_t *digest
+///      )
 assume val diceSHA256_2
-  (size1 : nat)
-  (data1: B.lbuffer uint8 size1)
-  (size2 : nat)
-  (data2 : B.lbuffer uint8 size2)
+  (#size1 : nat)
+  (data1: B.lbuffer HI.uint8 size1)
+  (#size2 : nat)
+  (data2 : B.lbuffer HI.uint8 size2)
   (digest: hash_t SHA2_256)
 : HST.Stack unit
   (requires fun h ->
@@ -94,4 +124,10 @@ assume val diceSHA256_2
     /\ B.disjoint data2 digest)
   (ensures  fun h0 _ h1 ->
       B.modifies (B.loc_buffer digest) h0 h1)
-
+///      {
+///          DICE_SHA256_CONTEXT context;
+///          DICE_SHA256_Init(&context);
+///          DICE_SHA256_Update(&context, buf1, bufSize1);
+///          DICE_SHA256_Update(&context, buf2, bufSize2);
+///          DICE_SHA256_Final(&context, digest);
+///      }
